Remove Throw from Free. Refactor IO.Free. Add io_try_catch_finnaly

Common.fst
@@ -13,17 +13,60 @@ let compose #a #b #c (g:b->c) (f:a->b) = fun x -> g (f x)
 let id #a (x:a) = x
 
 unfold let inl_app #a #b (f:a -> b) : maybe a -> maybe b =
-  fun x -> 
+  fun x ->
     match x with
     | Inl x -> Inl (f x)
     | Inr err -> Inr err
 
-  
+
 let cdr #a (_, (x:a)) : a = x
 
-let elim_pure #a #wp ($f : unit -> PURE a wp) p
- : Pure a (requires (wp p)) (ensures (fun r -> p r))
- //: PURE a (fun p' -> wp p /\ (forall r. p r ==> p' r))
- // ^ basically this, requires monotonicity
- = FStar.Monotonic.Pure.wp_monotonic_pure ();
-   f ()
+let elim_pure #a #wp ($f : unit -> PURE a wp) p :
+  Pure a (requires (wp p)) (ensures (fun r -> p r)) =
+  //: PURE a (fun p' -> wp p /\ (forall r. p r ==> p' r))
+  // ^ basically this, requires monotonicity
+  FStar.Monotonic.Pure.wp_monotonic_pure ();
+  f ()
+
+let rec prefix_of (l1 l2: list 'a)
+: Tot Type0 (decreases l2)
+= match l1, l2 with
+  | [], [] -> True
+  | [], _ -> True
+  | _, [] -> False
+  | h1 :: t1, h2 :: t2 -> h1 == h2 /\ t1 `prefix_of` t2
+
+let rec prefix_of_length (l1 l2: list 'a)
+: Lemma
+  (requires (prefix_of l1 l2))
+  (ensures (List.length l1 <= List.length l2))
+  (decreases l1)
+= match l1, l2 with
+  | h1 :: t1, h2 :: t2 ->
+    prefix_of_length t1 t2
+  | _ -> ()
+
+let rec suffix_of (l1 l2: list 'a)
+: Tot Type0 (decreases l2)
+= l1 == l2 \/ (match l2 with
+  | [] -> False
+  | _ :: q ->  l1 `suffix_of` q)
+
+let rec suffix_of_length (l1 l2: list 'a)
+: Lemma
+  (requires (suffix_of l1 l2))
+  (ensures (List.length l1 <= List.length l2))
+  (decreases l2) =
+  admit ()
+
+let suffix_of_append () :
+  Lemma (forall h l1 l2. suffix_of h ((List.rev l1) @ (List.rev l2) @ h)) =
+  admit()
+
+val rev_nil : (a:Type) -> Lemma (List.rev #a [] == [])
+let rev_nil a = ()
+
+val append_rev: l1:list 'a -> l2:list 'a ->
+  Lemma (
+    ((List.rev l1)@(List.rev l2)) == (List.rev (l2@l1)))
+let append_rev l1 l2 = List.rev_append l2 l1
