IO.Free.fst
@@ -3,30 +3,51 @@ module IO.Free
 open Common
 include Free
 
-type cmds = | Openfile | Read | Close | GetTrace
+type cmds = | Openfile | Read | Close | Throw | GetTrace
 
-// Observable actions
-type io_cmds = x:cmds{x = Openfile || x = Read || x = Close}
+(** Wish: It would be nice to define exn on top of free, and after
+that to define io on top of exn, but we use this big cmds with
+refeniments, therefore we have to make a monolith **)
 
-let io_sig : cmd_sig io_cmds = {
-  args = (fun (x:io_cmds) -> match x with
-    | Openfile -> string
-    | Read -> file_descr
-    | Close -> file_descr);
-  res = (fun (x:io_cmds) -> match x with
-    | Openfile -> file_descr
-    | Read -> string
-    | Close -> unit)
-}
+(** This steps are observable and produce events **)
+let _obs_cmds x = x = Openfile || x = Read || x = Close
 
-(** It is obvious that the primitives have no reason to throw
+(** Silent steps refer to the impossibility of an observer to see
+them. **)
+let _tau_cmds x = x = Throw
+
+type obs_cmds = x:cmds{_obs_cmds x}
+type tau_cmds = x:cmds{_tau_cmds x}
+
+(** the io free monad does not contain the GetTrace step **)
+type io_cmds = x:cmds{_obs_cmds x || _tau_cmds x}
+
+unfold let io_res (cmd:io_cmds) : Type =
+  match cmd with
+  | Openfile -> file_descr
+  | Read -> string
+  | Close -> unit
+  | Throw -> unit
+
+(** The IO primitives have no reason to throw
 `Contract_failure`, because they do not enforce any policy.
 In practice, a primitive can throw any error, but I think
 this is an assumption we can make to have more precise specification.
-`Contract_failure` is an exception defined by us in `Common.fst` **)
+`Contract_failure` is an exception defined in `Common.fst` **)
+unfold let io_resm (cmd:io_cmds) =
+  r:(maybe (io_res cmd))
+    {~(Inr? r /\ Inr?.v r == Contract_failure)}
+
+let io_sig : cmd_sig io_cmds = {
+  args = (fun (cmd:io_cmds) -> match cmd with
+    | Openfile -> string
+    | Read -> file_descr
+    | Close -> file_descr
+    | Throw -> exn);
+  res = io_resm
+}
+
 unfold let io_args (op:io_cmds) : Type = io_sig.args op
-unfold let io_res (op:io_cmds) = io_sig.res op
-unfold let io_resm (op:io_cmds) = r:(maybe (io_sig.res op)){~(Inr? r /\ Inr?.v r == Contract_failure)}
 
 noeq
 type event =
@@ -36,12 +57,7 @@ type event =
 
 type trace = list event
 
-// silent actions/steps
-(** Silent steps refer to the impossibility of an observer to see
-them. Two computations, one that uses GetTrace and does some IO,
-and another that does directly the same IO thing without playing
-with the trace, are equivalent from the observer point of view. **)
-type tau_cmds = x:cmds{x = GetTrace}
+type internal_cmds = x:cmds{x = GetTrace}
 
 (** We only need GetTrace because we assume that our actions are
 updating the trace for us. Therefore, at extraction, our actions
@@ -55,45 +71,82 @@ to the trace from the heap. **)
 at extraction, they have to be careful to link it directly with the
 primitives, and not with the wrapped version, otherwise, they will
 suffer a performance penalty. **)
-let tau_sig : cmd_sig tau_cmds = {
-  args = (fun (x:tau_cmds) -> match x with
+let internal_res (x:internal_cmds) =
+  match x with
+  | GetTrace -> list event
+let internal_resm (x:internal_cmds) = maybe (internal_res x)
+
+let internal_sig : cmd_sig internal_cmds = {
+  args = (fun (x:internal_cmds) -> match x with
     | GetTrace -> unit) ;
-  res = (fun (x:tau_cmds) -> match x with
-    | GetTrace -> list event)
+  res = internal_resm
 }
 
-let add_sig
-  (#p:cmds -> bool)
-  (#q:cmds -> bool)
-  (s1:cmd_sig (x:cmds{p x}))
-  (s2:cmd_sig (x:cmds{q x})) :
-  Tot (cmd_sig (y:cmds{p y || q y})) = {
-    args = (fun (x:cmds{p x || q x}) -> if p x then s1.args x else s2.args x);
-    res = (fun (x:cmds{p x || q x}) -> if p x then s1.res x else s2.res x)
-  }
+let all_sig = add_sig cmds io_sig internal_sig
 
-let all_sig = add_sig io_sig tau_sig
+unfold let args (cmd:cmds) : Type = all_sig.args cmd
+unfold let res (cmd:cmds)  : Type =
+  if cmd = GetTrace then internal_res cmd
+  else io_res cmd
 
-unfold let args (op:cmds) : Type = all_sig.args op
-unfold let res (op:cmds)  : Type = all_sig.res op
-unfold let resm (op:cmds) : Type = maybe (all_sig.res op)
+unfold let resm (cmd:cmds) : Type = maybe (res cmd)
 
-type io = free io_cmds io_sig
-let io_return (a:Type) (x:a) : io a= free_return io_cmds io_sig a x
-let io_throw (a:Type) (x:exn) : io a= free_throw io_cmds io_sig a x
-let io_bind (a:Type) (b:Type) l k : io b = free_bind io_cmds io_sig a b l k
+type io a = free io_cmds io_sig (maybe a)
+let io_return (a:Type) (x:a) : io a =
+  free_return io_cmds io_sig (maybe a) (Inl x)
+let io_throw (a:Type) (x:exn) : io a =
+  free_return io_cmds io_sig (maybe a) (Inr x)
+
+let rec io_try_catch_finnaly
+  (a b:Type)
+  (try_block:io a)
+  (catch_block:exn -> io b)
+  (finnaly:a -> io b) :
+  Tot (io b) =
+  match try_block with
+  | Return (Inl x) -> finnaly x
+  | Return (Inr err) -> catch_block err
+  | Call cmd argz fnc ->
+      Call cmd argz (fun res ->
+        io_try_catch_finnaly a b (fnc res) catch_block finnaly)
+
+let io_bind (a:Type) (b:Type) l k : io b =
+  io_try_catch_finnaly a b l (io_throw b) k
 
 let io_call (cmd:io_cmds) (arg:io_args cmd) : io (io_res cmd) =
-  free_perform (Call cmd arg Return)
+  Call cmd arg (fun v ->
+    match v with
+    | Inl x -> io_return (io_res cmd) x
+    | Inr err -> io_throw (io_res cmd) err)
 
 // THE IIO FREE MONAD
-type iio = free cmds all_sig
-let iio_return (a:Type) (x:a) : iio a = free_return cmds all_sig a x
-let iio_throw (a:Type) (x:exn) : iio a = free_throw cmds all_sig a x
-let iio_bind (a:Type) (b:Type) l k : iio b = free_bind cmds all_sig a b l k
+type iio a = free cmds all_sig (maybe a)
+let iio_return (a:Type) (x:a) : iio a =
+  free_return cmds all_sig (maybe a) (Inl x)
+let iio_throw (a:Type) (x:exn) : iio a =
+  free_return cmds all_sig (maybe a) (Inr x)
+
+let rec iio_try_catch_finnaly
+  (a b:Type)
+  (try_block:iio a)
+  (catch_block:exn -> iio b)
+  (finnaly:a -> iio b) :
+  Tot (iio b) =
+  match try_block with
+  | Return (Inl x) -> finnaly x
+  | Return (Inr err) -> catch_block err
+  | Call cmd argz fnc ->
+      Call cmd argz (fun res ->
+        iio_try_catch_finnaly a b (fnc res) catch_block finnaly)
+
+let iio_bind (a:Type) (b:Type) l k : iio b =
+  iio_try_catch_finnaly a b l (iio_throw b) k
 
 let iio_call (cmd:cmds) (arg:args cmd) : iio (res cmd) =
-  free_perform (Call cmd arg Return)
+  Call cmd arg (fun (v:(maybe (res cmd))) ->
+    match v with
+    | Inl x -> iio_return (res cmd) x
+    | Inr err -> iio_throw (res cmd) err)
 
 // OTHER TYPES & UTILS
 type action_type = (cmd : io_cmds) & (args cmd)
@@ -106,7 +159,10 @@ let convert_event_to_action (e:event) : action_type =
   | ERead arg _ -> (| Read, arg |)
   | EClose arg _ -> (| Close, arg |)
 
-let convert_call_to_event (cmd:io_cmds) (arg:io_args cmd) (r:io_resm cmd) =
+let convert_call_to_event
+  (cmd:obs_cmds)
+  (arg:io_args cmd)
+  (r:io_resm cmd) =
   match cmd with
   | Openfile -> EOpenfile arg r
   | Read -> ERead arg r
@@ -140,12 +196,6 @@ let rev_append_rev_append () : Lemma (
       ((List.rev (le1@le2)) @ h))
    by (FStar.Tactics.Derived.l_to_r [`List.append_assoc;`List.rev_append])
       = ()
-
-val rev_append_rev_append_pat_nil : h:trace ->
-  Lemma
-   (ensures ((List.rev #event []) @ h == h))
-   [SMTPat ((List.rev #event []) @ h)]
-let rev_append_rev_append_pat_nil h = rev_append_rev_append ()
 
 unfold
 let apply_changes (history local_events:trace) : Tot trace =
