Free.fst
@@ -1,19 +1,26 @@
 module Free
 
-open Common
-
 noeq
 type cmd_sig (op:Type u#a) = {
   args:(op -> Type u#a);
   res:(op -> Type u#a);
 }
 
+let add_sig
+  (cmds:Type)
+  (#p:cmds -> bool)
+  (#q:cmds -> bool)
+  (s1:cmd_sig (x:cmds{p x}))
+  (s2:cmd_sig (x:cmds{q x})) :
+  Tot (cmd_sig (y:cmds{p y || q y})) = {
+    args = (fun (x:cmds{p x || q x}) -> if p x then s1.args x else s2.args x);
+    res = (fun (x:cmds{p x || q x}) -> if p x then s1.res x else s2.res x)
+  }
+
 noeq
 type free (op:Type u#o) (s:cmd_sig op) (a:Type u#a) : Type u#(max o a) =
-  | Call : (l:op) -> (s.args l) -> cont:(maybe (s.res l) -> (free op s a)) -> free op s a
+  | Call : (l:op) -> (s.args l) -> cont:(s.res l -> (free op s a)) -> free op s a
   | Return : a -> free op s a
-  // TODO: is this relevant? can be made a silent cmd
-  | Throw : exn -> free op s a
 
 let free_codomain_ordering
   (#op:Type)
@@ -22,10 +29,8 @@ let free_codomain_ordering
   (x:(free op s a){Call? x}) :
   Lemma (forall r. Call?.cont x r << x) = ()
 
-let free_return (op:Type) (s:cmd_sig op) (a:Type) (x:a)   : free op s a =
+let free_return (op:Type) (s:cmd_sig op) (a:Type) (x:a) : free op s a =
   Return x
-let free_throw  (op:Type) (s:cmd_sig op) (a:Type) (x:exn) : free op s a =
-  Throw x
 
 let rec free_bind
   (op:Type u#o)
@@ -37,32 +42,9 @@ let rec free_bind
   Tot (free op s b) =
   match l with
   | Return x -> k x
-  | Throw err -> Throw err
   | Call cmd args fnc ->
       Call cmd args (fun i ->
         free_bind op s a b (fnc i) k)
-
-val lift_error :
-  (#op:Type) ->
-  (#s:cmd_sig op) ->
-  (#a:Type) ->
-  (maybe a) ->
-  Tot (free op s a)
-let lift_error #op #s #a v =
-  match v with
-  | Inl x -> free_return op s a x
-  | Inr err -> free_throw op s a err
-
-val free_perform :
-  (#op:Type) ->
-  (#s:cmd_sig op) ->
-  (#a:Type) ->
-  free op s (maybe a) ->
-  Tot (free op s a)
-let free_perform #op #s #a v =
-  free_bind op s (maybe a) (a)
-    v
-    lift_error
 
 let free_map
   (op:Type u#o)
